\documentclass{article}
\usepackage{ifthen}
\usepackage{epsfig}
\usepackage[utf8]{inputenc}
% Packages requested by user
\usepackage{stmaryrd}
\usepackage{amsmath}

\usepackage{newunicodechar}
  \newunicodechar{⁻}{${}^{-}$}% Superscript minus
  \newunicodechar{²}{${}^{2}$}% Superscript two
  \newunicodechar{³}{${}^{3}$}% Superscript three

\pagestyle{empty}
\begin{document}
$i>j$
\pagebreak

$T_{i,j} = 0$
\pagebreak

$i<j$
\pagebreak

$j>n-i-1$
\pagebreak

$j<n-i-1$
\pagebreak

$T_{i,i} = 1$
\pagebreak

$C = \alpha \mathrm{op}(A) \times \mathrm{op}(B)$
\pagebreak

$\mathrm{op}(A)=A^t$
\pagebreak

$\mathrm{op}(A)=A$
\pagebreak

$\mathrm{op}(A)$
\pagebreak

$m \times k$
\pagebreak

$\mathrm{op}(B)$
\pagebreak

$k \times n$
\pagebreak

$C$
\pagebreak

$m \times n$
\pagebreak

$n$
\pagebreak

$x \gets  x mod F$
\pagebreak

$x \gets  y mod F$
\pagebreak

$x \gets - x$
\pagebreak

$x \gets - y$
\pagebreak

$A \gets 0 $
\pagebreak

$A \gets random $
\pagebreak

$X = 0 $
\pagebreak

$X = Y $
\pagebreak

$x \gets y $
\pagebreak

$x \gets \alpha \cdot x$
\pagebreak

$y \gets \alpha \cdot x$
\pagebreak

$y \gets \alpha \cdot x + y$
\pagebreak

$y \gets \alpha \cdot x + \beta \cdot y$
\pagebreak

$x^T  y$
\pagebreak

$ X \leftrightarrow Y$
\pagebreak

$n^2$
\pagebreak

$A \gets B $
\pagebreak

$A = B $
\pagebreak

$A = 0 $
\pagebreak

$A \gets  A mod F$
\pagebreak

$A \gets  B mod F$
\pagebreak

$A \gets - A$
\pagebreak

$A \gets  - B$
\pagebreak

$A \gets a \cdot A$
\pagebreak

$B \gets a \cdot A$
\pagebreak

$ B \gets 0$
\pagebreak

$Y \gets \alpha \mathrm{op}(A) X + \beta Y $
\pagebreak

$A \gets \alpha x . y^T + A$
\pagebreak

$ X \gets \mathrm{op}(A^{-1}) X$
\pagebreak

$ X \gets \mathrm{op}(A) X$
\pagebreak

$\mathrm{op}(A)=A^T$
\pagebreak

$>n^2$
\pagebreak

$ B \gets \alpha \mathrm{op}(A^{-1}) B$
\pagebreak

$B \gets \alpha B \mathrm{op}(A^{-1})$
\pagebreak

$N\times N$
\pagebreak

$M\times M$
\pagebreak

$\alpha$
\pagebreak

$ B \gets \alpha \mathrm{op}(A) B$
\pagebreak

$B \gets \alpha B \mathrm{op}(A)$
\pagebreak

$ C \gets \alpha \mathrm{op}(A) B + beta C$
\pagebreak

$C \gets \alpha B \mathrm{op}(A) + beta C$
\pagebreak

$C = \alpha A \times A^T + \beta C$
\pagebreak

$C = \alpha A^T \times A + \beta C$
\pagebreak

$A$
\pagebreak

$n \times k$
\pagebreak

$n \times n$
\pagebreak

$C = \alpha A \times D \times A^T + \beta C$
\pagebreak

$C = \alpha A^T \times D \times A + \beta C$
\pagebreak

$ D\times A$
\pagebreak

$ A\times D$
\pagebreak

$D$
\pagebreak

$k \times k$
\pagebreak

$C = \alpha A \times Delta D \times A^T + \beta C$
\pagebreak

$C = \alpha A^T \times Delta D \times A + \beta C$
\pagebreak

$C = \alpha A Delta D \times A^T + \beta C$
\pagebreak

$C = \alpha A^T Delta D \times A + \beta C$
\pagebreak

$C = \alpha ( A \times B^T + B \times A^T) + \beta C$
\pagebreak

$C = \alpha ( A^T \times B + B^T \times A ) + \beta C$
\pagebreak

$C = \alpha ( A \times B^T + B \times A^T ) + \beta C$
\pagebreak

$C = \alpha ( A^T \times B + B^T \times A) + \beta C$
\pagebreak

$C = \alpha \mathrm{op}(A) \times \mathrm{op}(B) + \beta C$
\pagebreak

$ C \gets \alpha \mathrm{op}(A) \mathrm{op}(A) + \beta C$
\pagebreak

$A X = B$
\pagebreak

$X A = B$
\pagebreak

$ A = L \times D \times  L^T$
\pagebreak

$ A = U^T \times D \times  U$
\pagebreak

$ A = L \times Dinv \times  L^T$
\pagebreak

$2n^3$
\pagebreak

$M \times M$
\pagebreak

$A \gets A^{-1}$
\pagebreak

$ m \times m$
\pagebreak

$ \mathtt{nullity} = 0$
\pagebreak

$X = A^{-1}$
\pagebreak

$2n^3f$
\pagebreak

$ N \times N$
\pagebreak

$(v,Av, ..., A^Nv)$
\pagebreak

$ N \times (N+1)$
\pagebreak

$ r\times r$
\pagebreak

$ C \gets \alpha * A \times B + beta C $
\pagebreak

$ N \times s$
\pagebreak

$ (N - s) \times s$
\pagebreak

$ (N - ls) \times s$
\pagebreak

$ (N - s - ls) \times s$
\pagebreak

$ N \times t$
\pagebreak

$ N \times N $
\pagebreak

$ C \gets A \times B + beta C $
\pagebreak

$ Du + Tu  Su$
\pagebreak

$ Mu (Du + Tu  Su)$
\pagebreak

$ Dl + Sl  Tl $
\pagebreak

$(Dl + Tl Sl) Ml $
\pagebreak

$ \{0,\dots, N-1\}$
\pagebreak

\end{document}
